src/TotalMap.v
@@ -1,8 +1,9 @@
 From Coq Require Import ssreflect ssrfun ssrbool.
 Local Set Warnings "-notation-overridden".
-From mathcomp Require Import ssreflect.ssrnat.
-From Coq Require Export Arith.Arith Bool.Bool Strings.String.
+From mathcomp Require Import ssreflect.ssrnat eqtype.
+From Coq Require Export Arith.Arith Bool.Bool.
 From Coq Require Import Logic.FunctionalExtensionality.
+From PolyAI Require Export ssrstring.
 
 (* This code is inspired from the programming language fundations book *)
 
@@ -11,25 +12,24 @@ Local Open Scope list_scope.
 
 (* Representation of a total map with finite non-default values *)
 
-Inductive total_map (A: Type) :=
-| TEmpty (v: A)
-| TUpdate (m: total_map A) (x: string) (v: A)
+Inductive total_map {Key: eqType} {Value} :=
+| TEmpty (v: Value)
+| TUpdate (m: total_map) (k: Key) (v: Value)
 .
 
 (* Notation for a default map *)
-Notation "'_' '!->' v" := (TEmpty _ v)
+Notation "'_' '!->' v" := (TEmpty v)
   (at level 100, right associativity).
 
 (* Notation for a map update *)
-Notation "x '!->' v ';' m" := (TUpdate _ m x v)
+Notation "k '!->' v ';' m" := (TUpdate m k v)
                               (at level 100, v at next level, right associativity).
 
-
 (* Evaluate a map on a point*)
-Fixpoint eval_map {A: Type} (m: @total_map A) (x: string) :=
+Fixpoint eval_map {Key: eqType} {Value: Type} (m: @total_map Key Value) (k: Key) :=
   match m with
   | TEmpty v => v
-  | TUpdate m' x' v => if x' =? x then v else eval_map m' x
+  | TUpdate m' k' v => if k' == k then v else eval_map m' k
   end.
 
 (* Coercion for evaluation *)
@@ -37,102 +37,100 @@ Coercion eval_map : total_map >-> Funclass.
 
 (* Useful lemmas and theorems *)
 
-Lemma t_apply_empty : forall {A : Type} (x : string) (v : A),
-    (_ !-> v) x = v.
+Lemma t_apply_empty {Key: eqType} {Value: Type} (k: Key) (v: Value) :
+    (_ !-> v) k = v.
 Proof.
   by [].
 Qed.
 
-Lemma t_update_eq : forall {A : Type} (m : total_map A) (x: string) (v: A),
-    (x !-> v ; m) x = v.
+Lemma t_update_eq {Key : eqType} {Value: Type} (m : total_map) (k: Key) (v: Value) :
+    (k !-> v ; m) k = v.
 Proof.
-  move => A m x v /=.
-  by rewrite eqb_refl.
+  by rewrite /= eq_refl.
 Qed.
 
-Theorem t_update_neq : forall {A : Type} (m : total_map A) (x1 x2: string) (v: A),
-    x1 <> x2 ->
-    (x1 !-> v ; m) x2 = m x2.
+Theorem t_update_neq {Key: eqType} {Value : Type} (m : total_map) (k1 k2: Key) (v: Value) :
+    k1 != k2 ->
+    (k1 !-> v ; m) k2 = m k2.
 Proof.
-  by move => A m x1 x2 v /eqb_neq /= ->.
+  by move => /negb_true_iff /= ->.
 Qed.
 
-Lemma t_update_shadow : forall {A : Type} (m : total_map A) (x: string) (v1 v2: A),
-    eval_map (x !-> v2 ; x !-> v1 ; m) = eval_map (x !-> v2 ; m).
+Lemma t_update_shadow {Key: eqType} {Value: Type} (m : total_map) (k: Key) (v1 v2: Value) :
+    eval_map (k !-> v2 ; k !-> v1 ; m) = eval_map (k !-> v2 ; m).
 Proof.
-  move => A m x v1 v2 /=.
-  extensionality x'.
-  by case (x =? x').
+  extensionality k' => /=.
+  by case (k == k').
 Qed.
 
-Theorem t_update_same : forall {A : Type} (m : total_map A) (x: string),
-    eval_map (x !-> m x ; m) = eval_map m.
+Theorem t_update_same {Key : eqType} {Value: Type} (m : @total_map Key Value) (k: Key) :
+    eval_map (k !-> m k ; m) = eval_map m.
 Proof.
-  move => A m x /=.
-  extensionality x'.
-  by case (eqb_spec x x') => [<- | _].
+  extensionality k' => /=.
+  by case (k =P k') => [-> | ].
 Qed.
 
-Theorem t_update_permute : forall {A : Type} (m : total_map A)
-                                  (v1 v2: A) (x1 x2: string),
-    x2 <> x1 ->
-    eval_map (x1 !-> v1 ; x2 !-> v2 ; m) =
-    eval_map (x2 !-> v2 ; x1 !-> v1 ; m).
+Theorem t_update_permute {Key : eqType} {Value: Type} (m : total_map) (k1 k2: Key) (v1 v2: Value) :
+    k2 != k1 ->
+    eval_map (k1 !-> v1 ; k2 !-> v2 ; m) =
+    eval_map (k2 !-> v2 ; k1 !-> v1 ; m).
 Proof.
-  move => A m v1 v2 x1 x2 /eqb_neq Hne.
-  extensionality x'.
-  case (eqb_spec x1 x') => [ <- /= | /eqb_neq Hne' /= ].
-  - by rewrite eqb_refl Hne.
-  - by rewrite Hne'.
+  move => /negb_true_iff Hne /=.
+  extensionality k'.
+  case (k1 =P k') => [ <- /= | _ //].
+  - by rewrite Hne.
 Qed.
 
 Require Import Coq.ZArith.BinInt.
 
-Fixpoint pointwise_un_op {A B: Type} (m: total_map A) (f: A -> B) :=
+Fixpoint pointwise_un_op {Key: eqType} {Value Value': Type} (m: @total_map Key Value) (f: Value -> Value') :=
   match m with
-  | TEmpty x => (_ !-> f x)
-  | TUpdate m1' v x => let new_m := pointwise_un_op m1' f in
-                      (v !-> f x; new_m)
+  | TEmpty v => (_ !-> f v)
+  | TUpdate m1' k v => let new_m := pointwise_un_op m1' f in
+                      (k !-> f v; new_m)
   end.
 
-Theorem pointwise_un_op_spec {A B: Type} :
-  forall m (f: A -> B) v, (pointwise_un_op m f) v = f (m v).
+Theorem pointwise_un_op_spec {Key: eqType} {Value Value': Type} (m: @total_map Key Value) (f: Value -> Value') (k: Key) :
+  (pointwise_un_op m f) k = f (m k).
 Proof.
-  elim => [// | m Hind v x f v' /=].
+  elim: m f k => [// | m Hind k v f k' /=].
   rewrite Hind.
-    by case (v =? v').
+  by case (k == k').
 Qed.
 
-Fixpoint pointwise_bin_op_aux {A B C: Type} (m1: total_map A) (x2: B) (f: A -> B -> C) :=
+Fixpoint pointwise_bin_op_aux {Key: eqType} {Value1 Value2 Value3: Type} (m1: @total_map Key Value1)
+         (k2: Value2) (f: Value1 -> Value2 -> Value3) :=
   match m1 with
-  | TEmpty x1 => (_ !-> f x1 x2)
-  | TUpdate m1' v x1 => let new_m := pointwise_bin_op_aux m1' x2 f in
-                       (v !-> f x1 x2; new_m)
+  | TEmpty k1 => (_ !-> f k1 k2)
+  | TUpdate m1' v k1 => let new_m := pointwise_bin_op_aux m1' k2 f in
+                       (v !-> f k1 k2; new_m)
   end.
 
-Lemma pointwise_bin_op_aux_spec {A B C: Type} :
-  forall m1 x2 (f: A -> B -> C) s, (pointwise_bin_op_aux m1 x2 f) s = f (m1 s) x2.
+Lemma pointwise_bin_op_aux_spec {Key: eqType} {Value1 Value2 Value3: Type} (m1: @total_map Key Value1)
+      (v2: Value2) (f: Value1 -> Value2 -> Value3) (k: Key):
+  (pointwise_bin_op_aux m1 v2 f) k = f (m1 k) v2.
 Proof.
-  elim => [// | m H s x1 x2 f s' /=].
-  rewrite H.
-    by case (eqb_spec s s').
+  elim: m1 => [// | m1 Hind k1 v1 /=].
+  rewrite Hind.
+  by case (k1 == k).
 Qed.
 
-Fixpoint pointwise_bin_op {A B C: Type} (m1: total_map A) (m2: total_map B) (f: A -> B -> C) :=
+Fixpoint pointwise_bin_op {Key: eqType} {Value1 Value2 Value3: Type} (m1: @total_map Key Value1)
+         (m2: @total_map Key Value2) (f: Value1 -> Value2 -> Value3) :=
   match m2 with
-  | TEmpty x2 => pointwise_bin_op_aux m1 x2 f
-  | TUpdate m2' v x2 => let new_m := pointwise_bin_op m1 m2' f in
-                       (v !-> (f (m1 v) x2); new_m)
+  | TEmpty v2 => pointwise_bin_op_aux m1 v2 f
+  | TUpdate m2' k v2 => let new_m := pointwise_bin_op m1 m2' f in
+                       (k !-> (f (m1 k) v2); new_m)
   end.
 
-Theorem pointwise_bin_op_spec {A B C: Type} :
-  forall m1 m2 (f: A -> B -> C) x, (pointwise_bin_op m1 m2 f) x = f (m1 x) (m2 x).
+Theorem pointwise_bin_op_spec {Key: eqType} {Value1 Value2 Value3: Type} (m1: @total_map Key Value1)
+         (m2: @total_map Key Value2) (f: Value1 -> Value2 -> Value3) (k: Key):
+  (pointwise_bin_op m1 m2 f) k = f (m1 k) (m2 k).
 Proof.
-  move => m1 m2.
-  elim: m2 m1 => [v m1 f x | m Hind x v m1 f x0 /=].
+  elim: m2 m1 => [v m1 | m2 Hind k2 v2 m1 /=].
   - by apply pointwise_bin_op_aux_spec.
   - rewrite Hind.
-    case (eqb_spec x x0) => [ -> // | //].
+    by case (k2 =P k) => [-> // | //].
 Qed.
 
 Fixpoint list_string_in (l: list string) (s: string) :=
@@ -141,7 +139,7 @@ Fixpoint list_string_in (l: list string) (s: string) :=
   | s'::l' => (s =? s')%string || list_string_in l' s
   end.
 
-Theorem list_string_in_spec :
+Theorem list_string_in_spec:
   forall l s, reflect (List.In s l) (list_string_in l s).
 Proof.
   elim => [s // | a l Hind s /=].
@@ -235,95 +233,86 @@ Proof.
     by rewrite ltnn in HIn.
 Qed.
 
-Fixpoint forall_bin_op_aux {A: Type} (m1: total_map A) (x2: A) (f: A -> A -> bool) (seen: list string):=
+Fixpoint forall_bin_op_aux {Value: Type} (m1: total_map) (v2: Value)
+         (f: Value -> Value -> bool) (seen: list string) :=
   match m1 with
-  | TEmpty x1 => f x1 x2
-  | TUpdate m1' v x1 =>
-    if list_string_in seen v then
-      forall_bin_op_aux m1' x2 f seen
+  | TEmpty v1 => f v1 v2
+  | TUpdate m1' k v1 =>
+    if list_string_in seen k then
+      forall_bin_op_aux m1' v2 f seen
     else
-      f x1 x2 && forall_bin_op_aux m1' x2 f (v::seen)
+      f v1 v2 && forall_bin_op_aux m1' v2 f (k::seen)
   end.
 
-Lemma forall_bin_op_aux_spec {A: Type} :
-  forall m1 (x2: A) f seen, forall_bin_op_aux m1 x2 f seen <->
-                       (forall v, not (List.In v seen) -> f (m1 v) x2).
+Lemma forall_bin_op_aux_spec {Value: Type} {m1: total_map} (v2: Value)
+      (f: Value -> Value -> bool) (seen: list string) :
+  forall_bin_op_aux m1 v2 f seen <->
+                       (forall k, not (List.In k seen) -> f (m1 k) v2).
 Proof.
-  elim => [v x2 f seen /= | m Hind v x1 x2 f seen /=].
+  elim: m1 seen => [v seen /= | m Hind k v1 seen /=].
     by split => [// | H]; apply (H (construct_not_in_list seen)), construct_not_in_list_spec.
-  case (list_string_in seen v) eqn:Hseen.
+  case (list_string_in seen k) eqn:Hseen.
   - rewrite Hind.
-    split => [Hin v0 HnotIn| Hin v0 Hf].
-    + case (v =? v0) eqn: Hvv0; last first. by apply Hin.
-        by move: Hvv0 Hseen => /eqb_spec -> /list_string_in_spec Hseen.
-    + case (v =? v0) eqn: Hvv0; last first. apply Hin in Hf. by rewrite Hvv0 in Hf.
-        by move: Hvv0 Hseen => /eqb_spec -> /list_string_in_spec Hseen.
-  - split => [/andP[Hf /Hind Hforall] v0 Hv0notin | H ].
-    + case (v =? v0) eqn:Hvv0 => [// | ].
-      move: Hvv0 => /eqb_spec Hvv0.
+    split => [Hin k0 HnotIn| Hin k0 Hf].
+    + case (k == k0) eqn: Hkk0; last first. by apply Hin.
+        by move: Hkk0 Hseen => /eqb_spec -> /list_string_in_spec Hseen.
+    + case (k == k0) eqn: Hkk0; last first. apply Hin in Hf. by rewrite Hkk0 in Hf.
+        by move: Hkk0 Hseen => /eqb_spec -> /list_string_in_spec Hseen.
+  - split => [/andP[Hf /Hind Hforall] k0 Hk0notin | H ].
+    + case (k == k0) eqn:Hkk0 => [// | ].
+      move: Hkk0 => /eqb_spec Hkk0.
       apply Hforall.
       by case.
     + apply /andP. split.
       * move: Hseen => /list_string_in_spec Hseen.
         apply H in Hseen.
-          by rewrite eqb_refl in Hseen.
-      * apply Hind => v0 /= /Decidable.not_or [/eqb_spec Hvv0 Hnotin].
-        apply H in Hnotin.
-        rewrite /is_true in Hvv0.
-        apply negb_true_iff in Hvv0.
-          by rewrite Hvv0 in Hnotin.
+          by rewrite eq_refl in Hseen.
+      * apply Hind => k0 /= /Decidable.not_or [/eqP /negb_true_iff Hkk0 /H Hnotin].
+          by rewrite Hkk0 in Hnotin.
 Qed.
 
-Fixpoint forall_bin_op_fix {A: Type} (m1 m2: total_map A) (f: A -> A -> bool) (seen: list string):=
+Fixpoint forall_bin_op_fix {Value: Type} (m1 m2: total_map) (f: Value -> Value -> bool) (seen: list string):=
   match m2 with
-  | TEmpty x2 => forall_bin_op_aux m1 x2 f seen
-  | TUpdate m2' v x2 =>
-    if list_string_in seen v then
+  | TEmpty v2 => forall_bin_op_aux m1 v2 f seen
+  | TUpdate m2' k v2 =>
+    if list_string_in seen k then
       forall_bin_op_fix m1 m2' f seen
     else
-      f (m1 v) x2 && forall_bin_op_fix m1 m2' f (v::seen)
+      f (m1 k) v2 && forall_bin_op_fix m1 m2' f (k::seen)
   end.
 
-Lemma forall_bin_op_fix_spec {A: Type} :
-  forall (m1 m2: @total_map A) f seen, forall_bin_op_fix m1 m2 f seen <->
-                                  forall v, not (List.In v seen) -> f (m1 v) (m2 v).
+Lemma forall_bin_op_fix_spec {Value: Type} (m1 m2: total_map) (f: Value -> Value -> bool) (seen: list string) :
+  forall_bin_op_fix m1 m2 f seen <-> forall k, not (List.In k seen) -> f (m1 k) (m2 k).
 Proof.
-  move => m1 m2; move: m2 m1.
-  elim => [m1 m2 f seen /= | m2 Hind v x1 m1 f seen /=].
-    by split => /forall_bin_op_aux_spec //.
-  case (list_string_in seen v) eqn:Hseen; move: Hseen => /list_string_in_spec Hseen.
+  move: m2 m1 seen.
+  elim => [v1 m2 seen /= | m2 Hind k v1 m1 seen /=].
+    by split => /forall_bin_op_aux_spec.
+  case (list_string_in seen k) eqn:Hseen; move: Hseen => /list_string_in_spec Hseen.
   - rewrite Hind.
-    split => [Hin v0 HnotIn| Hin v0 Hf].
-    + case (v =? v0) eqn: Hvv0; last first. by apply Hin.
-        by move: Hvv0 Hseen => /eqb_spec ->.
-    + case (v =? v0) eqn: Hvv0; last first. apply Hin in Hf. by rewrite Hvv0 in Hf.
-        by move: Hvv0 Hseen => /eqb_spec ->.
-  - split => [/andP[Hf /Hind Hforall] v0 Hv0notin | H ].
-    + case (v =? v0) eqn:Hvv0 => [ | ].
-      * by move: Hvv0 => /eqb_spec <-.
-      * apply Hforall.
-        move: Hvv0 => /eqb_spec Hvv0.
-        by case.
+    split => [Hin k0 HnotIn| Hin k0 Hf].
+    + case (k == k0) eqn: Hkk0; last first. by apply Hin.
+        by move: Hkk0 Hseen => /eqb_spec ->.
+    + case (k == k0) eqn: Hkk0; last first. apply Hin in Hf. by rewrite Hkk0 in Hf.
+        by move: Hkk0 Hseen => /eqb_spec ->.
+  - split => [/andP[Hf /Hind Hforall] k0 Hk0notin | H ].
+    + case_eq (k == k0) => [ /eqP <- // | /eqP Hkk0 ].
+      apply Hforall.
+      by case.
     + apply /andP. split.
       * apply H in Hseen.
-          by rewrite eqb_refl in Hseen.
-      * apply Hind => v0 /= /Decidable.not_or [/eqb_spec Hvv0 Hnotin].
-        apply H in Hnotin.
-        rewrite /is_true in Hvv0.
-        apply negb_true_iff in Hvv0.
+          by rewrite eq_refl in Hseen.
+      * apply Hind => v0 /= /Decidable.not_or [/eqP /negb_true_iff Hvv0 /H Hnotin].
           by rewrite Hvv0 in Hnotin.
 Qed.
 
-Definition forall_bin_op {A: Type} (m1 m2: total_map A) (f: A -> A -> bool) :=
+Definition forall_bin_op {Value: Type} (m1 m2: total_map) (f: Value -> Value -> bool) :=
   forall_bin_op_fix m1 m2 f nil.
 
-Theorem forall_bin_op_spec {A: Type} :
-  forall (m1 m2: @total_map A) f, forall_bin_op m1 m2 f <-> forall v, f (m1 v) (m2 v).
+Theorem forall_bin_op_spec {Value: Type} (m1 m2: total_map) (f: Value -> Value -> bool) :
+  forall_bin_op m1 m2 f <-> forall k, f (m1 k) (m2 k).
 Proof.
-  move => m1 m2 f.
-  unfold forall_bin_op.
   rewrite forall_bin_op_fix_spec /=.
-  split => [H | H v _].
+  split => [H // | H k _].
   - auto.
   - by apply H.
 Qed.
@@ -333,19 +322,19 @@ Qed.
 Ltac simpl_totalmap :=
 repeat match goal with
        | [ |- context[eval_map (_ !-> _) _] ] => rewrite t_apply_empty
-       | [ |- context[eval_map (?v !-> _ ; _) ?v]] => rewrite t_update_eq
-       | [ H : ?v1 <> ?v2 |- context[eval_map (?v1 !-> _ ; _) ?v2] ] => rewrite (t_update_neq _ _ _ _ H)
-       | [ |- context[eval_map (?v1 !-> _ ; ?m) ?v2]] => rewrite (t_update_neq m v1 v2 _); last first; [ by apply eqb_neq | idtac ]
-       | [ |- context[eval_map (?v !-> _ ; ?v !-> _ ; _)]] => rewrite t_update_shadow
-       | [ |- context[eval_map (?x !-> eval_map ?m ?x ; ?m)]] => rewrite t_update_same
-       | [ |- context[(?s =? ?s)%string]] => rewrite eqb_refl
+       | [ |- context[eval_map (?k !-> _ ; _) ?k]] => rewrite t_update_eq
+       | [ H : ?k1 <> ?k2 |- _ ] => move: H => /eqP H
+       | [ H : ?k1 != ?k2 |- context[eval_map (?k1 !-> _ ; _) ?k2] ] => rewrite (t_update_neq _ _ _ _ H)
+       | [ |- context[eval_map (?k1 !-> _ ; ?m) ?k2]] => rewrite (t_update_neq m k1 k2 _); last first; [ by [] | idtac ]
+       | [ |- context[eval_map (?k !-> _ ; ?k !-> _ ; _)]] => rewrite t_update_shadow
+       | [ |- context[eval_map (?k !-> eval_map ?m ?k ; ?m)]] => rewrite t_update_same
+       | [ |- context[(?k == ?k)]] => rewrite eq_refl
        | [ |- context[eval_map (pointwise_un_op _ _) _]] => rewrite pointwise_un_op_spec
        | [ |- context[eval_map (pointwise_bin_op _ _ _) _]] => rewrite pointwise_bin_op_spec
        | [ |- is_true (forall_bin_op _ _ _)] => apply forall_bin_op_spec
+       | [ H : is_true ?x |- context[?x]] => rewrite H
+       | [ H : is_true (?x != ?y) |- context[?x == ?y]] => rewrite ?(ifN_eq _ _ H) ?(ifN_eqC _ _ H)
        | _ => rewrite /=
        end.
-
-Ltac simpl_totalmap_Z :=
-  repeat ( simpl_totalmap; rewrite ?Z.eqb_refl ).
 
 Global Opaque eval_map.
