src/ssrZ.v
@@ -1,0 +1,6 @@
+Local Set Warnings "-notation-overridden".
+From mathcomp Require Export eqtype.
+Require Export Coq.ZArith.BinInt.
+
+Canonical Z_eqMixin := EqMixin Z.eqb_spec.
+Canonical Z_eqType := Eval hnf in EqType Z Z_eqMixin.
