src/ssrstring.v
@@ -1,0 +1,19 @@
+From Coq Require Import ssreflect ssrfun ssrbool.
+From Coq Require Export Strings.String.
+Local Set Warnings "-notation-overridden".
+From mathcomp Require Export eqtype.
+
+Local Open Scope string_scope.
+
+Lemma eqstringP : Equality.axiom String.eqb.
+Proof.
+  rewrite /Equality.axiom.
+  elim => [ | a s Hind]; case => [ | a0 s0]; apply (iffP idP) => //.
+  - simpl.
+      by case_eq (Ascii.eqb a a0) => [/Ascii.eqb_eq -> /eqb_spec -> | ].
+  - move ->.
+      by apply eqb_refl.
+Qed.
+
+Canonical string_eqMixin := EqMixin eqstringP.
+Canonical string_eqType := Eval hnf in EqType string string_eqMixin.
